@prefix :        <http://www.owl-ontologies.com/StoryWorldSettings/plop.owl#> .
@prefix ns1:     <http://www.owl-ontologies.com/StoryWorldCore.owl#> .
@prefix rdfs:    <http://www.w3.org/2000/01/rdf-schema#> .
@prefix ns0:     <http://www.owl-ontologies.com/FabulaKnowledge.owl#> .
@prefix owl:     <http://www.w3.org/2002/07/owl#> .
@prefix rdf:     <http://www.w3.org/1999/02/22-rdf-syntax-ns#> .

<plop.owl> {
	fabula:Taste
          a       owl:Class ;
          rdfs:subClassOf fabula:Perception .

    fabula:Drink
          a       owl:Class ;
          rdfs:comment "Ingesting substance food." ;
          rdfs:subClassOf fabula:Consume .

    fabula:duration
          a       owl:DatatypeProperty , owl:FunctionalProperty ;
          rdfs:comment "total duration of an action" ;
          rdfs:domain fabula:Action ;
          rdfs:range <http://www.w3.org/2001/XMLSchema#string> .

    fabula:Close
          a       owl:Class ;
          rdfs:comment "Close a device which is open and can be closed using the object itself. This excludes closing a frying pan with its cover, assuming that the cover is not a part of the pan." ;
          rdfs:subClassOf fabula:Manipulate .

    fabula:Feel
          a       owl:Class ;
          rdfs:subClassOf fabula:Perception .

    fabula:Insert
          a       owl:Class ;
          rdfs:comment "The action of inserting an Object into another object." ;
          rdfs:subClassOf fabula:Put .

    fabula:character
          a       owl:FunctionalProperty , owl:ObjectProperty ;
          rdfs:domain fabula:FabulaElement .

    fabula:chanceOfSuccess
          a       owl:DatatypeProperty , owl:FunctionalProperty ;
          rdfs:comment "Chance of success for an action" ;
          rdfs:domain fabula:Action ;
          rdfs:range <http://www.w3.org/2001/XMLSchema#string> .

    fabula:Fold
          a       owl:Class ;
          rdfs:comment "Fold a foldable item into its folded or original state." ;
          rdfs:subClassOf fabula:Manipulate .

    fabula:Walk
          a       owl:Class ;
          rdfs:comment "Normal movement over ground." ;
          rdfs:subClassOf fabula:Ambulate .

    fabula:Unlock
          a       owl:Class ;
          rdfs:comment "Unlock a lock with a key." ;
          rdfs:subClassOf fabula:Manipulate .

    <http://www.owl-ontologies.com/FabulaKnowledge.owl>
          a       owl:Ontology ;
          owl:imports <http://protege.stanford.edu/plugins/owl/protege> .

    fabula:AvoidGoal
          a       owl:Class ;
          rdfs:comment "A goal to avoid a certain situation / state, i.e. that the vilain escapes" ;
          rdfs:subClassOf fabula:Goal .

    fabula:Disassemble
          a       owl:Class ;
          rdfs:comment "Disassemble the object into its parts." ;
          rdfs:subClassOf fabula:Creation .

    fabula:Cognition
          a       owl:Class ;
          rdfs:subClassOf fabula:InternalElement .

    fabula:WorldChanges
          a       owl:Class ;
          rdfs:subClassOf fabula:InternalAttribute .

    fabula:motivates
          a       owl:ObjectProperty ;
          rdfs:subPropertyOf fabula:causes .

    fabula:TestMove1Effects
          a       fabula:TestMoveEffects ;
          fabula:delete "(swc:isMovingOnTransitWay ?AGENS ?path)" .

    fabula:Drain
          a       owl:Class ;
          rdfs:comment "Using a syringe to extract a Substance from an Object. Inverse (more or less) of Inject." ;
          rdfs:subClassOf fabula:Extract .

    fabula:BeliefElement
          a       owl:Class ;
          rdfs:comment "An Internal Element representing a belief of a character" ;
          rdfs:subClassOf fabula:InternalElement .

    fabula:Goal
          a       owl:Class ;
          rdfs:comment "A goal of a character" ;
          rdfs:subClassOf fabula:FabulaElement .

    fabula:Event
          a       owl:Class ;
          rdfs:comment "Any change in the world that is not a direct and planned result of a character action" ;
          rdfs:subClassOf fabula:FabulaElement .

    fabula:Outcome
          a       owl:Class ;
          rdfs:comment "Describes what happened to a Goal" ;
          rdfs:subClassOf fabula:FabulaElement .

    fabula:resolves
          a       owl:ObjectProperty , owl:FunctionalProperty ;
          rdfs:domain fabula:Outcome ;
          rdfs:range fabula:Goal .

    fabula:TestMoveInterEffects
          a       owl:Class ;
          rdfs:subClassOf fabula:TestMoveChanges ;
          rdfs:subClassOf
                  [ a       owl:Restriction ;
                    owl:hasValue "(swc:supportedBy ?AGENS ?currLoc)" ;
                    owl:onProperty fabula:delete
                  ] .

    fabula:enables
          a       owl:ObjectProperty ;
          rdfs:subPropertyOf fabula:causes .

    fabula:TestMove
          a       owl:Class ;
          rdfs:comment "A testing move. Should be removed if everything is working properly." ;
          rdfs:subClassOf fabula:Action ;
          rdfs:subClassOf
                  [ a       owl:Restriction ;
                    owl:hasValue "100" ;
                    owl:onProperty fabula:chanceOfSuccess
                  ] ;
          rdfs:subClassOf
                  [ a       owl:Restriction ;
                    owl:hasValue "2" ;
                    owl:onProperty fabula:interruptableDuration
                  ] ;
          rdfs:subClassOf
                  [ a       owl:Restriction ;
                    owl:hasValue "(rdf:type ?currLoc swc:GeographicArea)" ;
                    owl:onProperty fabula:preconditions
                  ] ;
          rdfs:subClassOf
                  [ a       owl:Restriction ;
                    owl:hasValue "4" ;
                    owl:onProperty fabula:duration
                  ] ;
          rdfs:subClassOf
                  [ a       owl:Restriction ;
                    owl:hasValue "(swc:supportedBy ?AGENS ?currLoc)" ;
                    owl:onProperty fabula:preconditions
                  ] .

    fabula:StitchOff
          a       owl:Class ;
          rdfs:comment "Turn off a device which 'on'." ;
          rdfs:subClassOf fabula:Manipulate .

    <http://www.owl-ontologies.com/FabulaKnowledge.owl#ind_See.plop.12>
          a       fabula:See ;
          fabula:character <http://www.owl-ontologies.com/StoryWorldCore.owl#ind_Humanoid.plop.1> ;
          fabula:psi_causes <http://www.owl-ontologies.com/FabulaKnowledge.owl#ind_BeliefElement.plop.14> .

    fabula:causes
          a       owl:ObjectProperty .

    <http://www.owl-ontologies.com/FabulaKnowledge.owl#ind_Eat.plop.9>
          a       fabula:Eat ;
          fabula:agens <http://www.owl-ontologies.com/StoryWorldCore.owl#ind_Humanoid.plop.1> ;
          fabula:hasContext <http://www.owl-ontologies.com/StoryWorldCore.owl#ind_AttainGoal.plop.8> ;
          fabula:patiens <http://www.owl-ontologies.com/StoryWorldCore.owl#ind_FruitOrVegetable.plop.6> .

    fabula:FutureBeliefElement
          a       owl:Class ;
          rdfs:comment "Describes a belief about the future, this could be a hope or a worry, for instance" ;
          rdfs:subClassOf fabula:BeliefElement .

    fabula:TakeFrom
          a       owl:Class ;
          rdfs:comment """The action of taking an object which is supported by another
object.""" ;
          rdfs:subClassOf fabula:Take .

    fabula:SwitchOn
          a       owl:Class ;
          rdfs:comment "Turn a device with a power source on." ;
          rdfs:subClassOf fabula:Manipulate .

    fabula:Consume
          a       owl:Class ;
          rdfs:comment "Ingesting food" ;
          rdfs:subClassOf fabula:Action .

    fabula:Smell
          a       owl:Class ;
          rdfs:subClassOf fabula:Perception .

    fabula:preconditions
          a       owl:DatatypeProperty ;
          rdfs:comment "Conditions which must hold for an action to be performed" ;
          rdfs:domain fabula:Action ;
          rdfs:range <http://www.w3.org/2001/XMLSchema#string> .

    fabula:Character
          a       owl:Class .

    fabula:InternalElement
          a       owl:Class ;
          rdfs:comment "Anything internal to a character, like a belief, or an emotion, feeling, etc." ;
          rdfs:subClassOf fabula:FabulaElement .

    fabula:Extract
          a       owl:Class ;
          rdfs:comment "The action of extracting an Object from another Object" ;
          rdfs:subClassOf fabula:Take .

    fabula:Creation
          a       owl:Class ;
          rdfs:comment "Class of actions dealing with creation and uncreation." ;
          rdfs:subClassOf fabula:Action .

    fabula:interEffects
          a       owl:ObjectProperty , owl:FunctionalProperty ;
          rdfs:comment "Changes of the world after interDuration time has passed, and therefore making the action uninterruptable. Only used in TransitMoves." ;
          rdfs:domain fabula:Action ;
          rdfs:range fabula:WorldChanges .

    fabula:Open
          a       owl:Class ;
          rdfs:comment "Open a device which is closed." ;
          rdfs:subClassOf fabula:Manipulate .

    <http://www.owl-ontologies.com/FabulaKnowledge.owl#ind_Outcome.plop.16>
          a       fabula:Outcome ;
          fabula:character <http://www.owl-ontologies.com/StoryWorldCore.owl#ind_Humanoid.plop.1> ;
          fabula:resolves <http://www.owl-ontologies.com/StoryWorldCore.owl#ind_AttainGoal.plop.8> .

    fabula:Transfer
          a       owl:Class ;
          rdfs:comment """The general action of changing the location of an object other
than the acting object.""" ;
          rdfs:subClassOf fabula:Action .

    fabula:PutIn
          a       owl:Class ;
          rdfs:comment "The action of placing an Object inside a Container." ;
          rdfs:subClassOf fabula:Insert .

    fabula:DropControl
          a       owl:Class ;
          rdfs:comment "Drop control over a device." ;
          rdfs:subClassOf fabula:ControlAct .

    fabula:TestMove2
          a       fabula:TestMove ;
          fabula:effects fabula:TestMove1Effects ;
          fabula:interEffects fabula:TestMove1InterEffects ;
          fabula:preconditions
                  "(swc:toGeographicArea ?path ?currLoc)" , "(swc:fromGeographicArea ?path ?TARGET)" .

    fabula:TestMove1InterEffects
          a       fabula:TestMoveInterEffects ;
          fabula:add "(swc:isMovingOnTransitWay ?AGENS ?path)" .

    fabula:add
          a       owl:DatatypeProperty ;
          rdfs:comment "List of facts to be added upon a world change." ;
          rdfs:domain fabula:WorldChanges ;
          rdfs:range <http://www.w3.org/2001/XMLSchema#string> .

    fabula:TestMove3
          a       fabula:TestMove ;
          fabula:effects fabula:TestMove1Effects ;
          fabula:interEffects fabula:TestMove1InterEffects ;
          fabula:preconditions
                  "(swc:toGeographicArea ?path ?TARGET)" , "(swc:fromGeographicArea ?path ?currloc)" , "(not(swc:attachedBy ?AGENS ?AttachingObject))" .

    fabula:TestMove4
          a       fabula:TestMove ;
          fabula:effects fabula:TestMove1Effects ;
          fabula:interEffects fabula:TestMove1InterEffects ;
          fabula:preconditions
                  "(swc:fromGeographicArea ?path ?currLoc)" , "(swc:toGeographicArea ?path ?TARGET)" , "(swc:isLocated ?TARGET ?multipleAnswers)" .

    <http://www.owl-ontologies.com/FabulaKnowledge.owl#ind_BeliefElement.plop.14>
          a       fabula:BeliefElement ;
          fabula:character <http://www.owl-ontologies.com/StoryWorldCore.owl#ind_Humanoid.plop.1> ;
          fabula:psi_causes <http://www.owl-ontologies.com/FabulaKnowledge.owl#ind_Outcome.plop.16> .

    fabula:Untie
          a       owl:Class ;
          rdfs:comment "Detaching an object which is fastened by a rope-like device." ;
          rdfs:subClassOf fabula:Detach .

    fabula:psi_causes
          a       owl:ObjectProperty ;
          rdfs:subPropertyOf fabula:causes .

    fabula:Action
          a       owl:Class ;
          rdfs:subClassOf fabula:FabulaElement .

    fabula:TestMoveEffects
          a       owl:Class ;
          rdfs:subClassOf fabula:TestMoveChanges ;
          rdfs:subClassOf
                  [ a       owl:Restriction ;
                    owl:hasValue "(swc:supportedBy ?AGENS ?TARGET)" ;
                    owl:onProperty fabula:add
                  ] .

    fabula:CurrentBeliefElement
          a       owl:Class ;
          rdfs:comment "Describes a belief about the now...e.g. what is believed to be true now." ;
          rdfs:subClassOf fabula:BeliefElement .

    fabula:effects
          a       owl:FunctionalProperty , owl:ObjectProperty ;
          rdfs:comment "effects of an succesfully performed action" ;
          rdfs:domain fabula:Action ;
          rdfs:range fabula:WorldChanges .

    fabula:Emotion
          a       owl:Class ;
          rdfs:subClassOf fabula:InternalElement .

    fabula:Detach
          a       owl:Class ;
          rdfs:subClassOf fabula:Attaching .

    fabula:TakeOut
          a       owl:Class ;
          rdfs:comment "The action of taking an object out of a Container." ;
          rdfs:subClassOf fabula:Extract .

    fabula:Eat
          a       owl:Class ;
          rdfs:comment "Ingesting corpuscular food. (i.e. food which is not a substance)." ;
          rdfs:subClassOf fabula:Consume .

    fabula:Glue
          a       owl:Class ;
          rdfs:comment "Attach one object to another using a sticky substance. The substance will be removed from the storyworld after use." ;
          rdfs:subClassOf fabula:Attach .

    fabula:TransitMove
          a       owl:Class ;
          rdfs:comment """The general class of actions in which the acting object changes
its location.""" ;
          rdfs:subClassOf fabula:Action .

    fabula:Assemble
          a       owl:Class ;
          rdfs:comment "Creating an artifact from its parts. Action is reversible by Disassemble." ;
          rdfs:subClassOf fabula:Make .

    fabula:Ambulate
          a       owl:Class ;
          rdfs:comment "Movement over ground using legs." ;
          rdfs:subClassOf fabula:GroundMove .

    fabula:Inject
          a       owl:Class ;
          rdfs:comment """Inserting a BiologicallyActiveSubstance into an Animal or Human
with a syringe. This is SUMO and will not be implemented in our first
world.""" ;
          rdfs:subClassOf fabula:Insert .

    fabula:isNonPerception
          a       owl:DatatypeProperty , owl:FunctionalProperty ;
          rdfs:domain fabula:Perception ;
          rdfs:range <http://www.w3.org/2001/XMLSchema#boolean> .

    <http://www.owl-ontologies.com/FabulaKnowledge.owl#ind_BeliefElement.plop.3>
          fabula:character <http://www.owl-ontologies.com/StoryWorldCore.owl#ind_Humanoid.plop.1> ;
          fabula:psi_causes <http://www.owl-ontologies.com/StoryWorldCore.owl#ind_AttainGoal.plop.8> .

    fabula:Fly
          a       owl:Class ;
          rdfs:comment """Movement through the air using wings. Is not yet different from Air-
Move. Note that AirMove is included because of consistency, and Fly is
added because it is a more intuitive term to use. One can split AirMove
in movement using moving wings and movement using a jet-engine, if
it proves to be a useful distinction.""" ;
          rdfs:subClassOf fabula:AirMove .

    fabula:Attaching
          a       owl:Class ;
          rdfs:comment "General class of actions that deal with attaching and detaching objects." ;
          rdfs:subClassOf fabula:Action .

    fabula:LeaveGoal
          a       owl:Class ;
          rdfs:comment "A goal to leave a certain situation / state, i.e. being hungry" ;
          rdfs:subClassOf fabula:Goal .

    fabula:TestMoveChanges
          a       owl:Class ;
          rdfs:subClassOf fabula:WorldChanges .

    fabula:Lock
          a       owl:Class ;
          rdfs:comment "Lock a securityDevice 'Lock'" ;
          rdfs:subClassOf fabula:Manipulate .

    fabula:TakeControl
          a       owl:Class ;
          rdfs:comment "Take control of a device." ;
          rdfs:subClassOf fabula:ControlAct .

    <http://www.owl-ontologies.com/StoryWorldCore.owl#ind_FruitOrVegetable.plop.6>
          a       ns1:FruitOrVegetable ;
          fabula:hasContext <http://www.owl-ontologies.com/FabulaKnowledge.owl#ind_BeliefElement.plop.3> ;
          fabula:hasInterpretation
                  <http://www.owl-ontologies.com/StoryWorldCore.owl#ind_FruitOrVegetable.plop.4> ;
          ns1:isLocated <http://www.owl-ontologies.com/StoryWorldCore.owl#ind_GeographicArea.plop.7> .

    <http://www.owl-ontologies.com/FabulaKnowledge.owl#ind_TakeFrom.plop.10>
          a       fabula:TakeFrom ;
          fabula:agens <http://www.owl-ontologies.com/StoryWorldCore.owl#ind_Humanoid.plop.1> ;
          fabula:patiens <http://www.owl-ontologies.com/StoryWorldCore.owl#ind_FruitOrVegetable.plop.6> .

    <http://www.owl-ontologies.com/StoryWorldCore.owl#ind_FruitOrVegetable.plop.4>
          a       ns1:FruitOrVegetable .

    <http://www.owl-ontologies.com/StoryWorldCore.owl#ind_AttainGoal.plop.8>
          a       ns1:AttainGoal ;
          fabula:character <http://www.owl-ontologies.com/StoryWorldCore.owl#ind_Humanoid.plop.1> ;
          fabula:motivates <http://www.owl-ontologies.com/FabulaKnowledge.owl#ind_TakeFrom.plop.10> , <http://www.owl-ontologies.com/FabulaKnowledge.owl#ind_Eat.plop.11> .

    fabula:WaterMove
          a       owl:Class ;
          rdfs:comment "All movement that is done over a WaterWay." ;
          rdfs:subClassOf fabula:TransitMove .

    fabula:Transform
          a       owl:Class ;
          rdfs:comment "Creating an artifact from its substances. (i.e. create a WineGlass from Sand or a Key from Metal). Action is irreversible." ;
          rdfs:subClassOf fabula:Make .

    fabula:Put
          a       owl:Class ;
          rdfs:comment """The action of changing the location of an object which has an isLocated
relation with the hands (or hand-like object) of the actor. After the
action the actor does not hold the object anymore.""" ;
          rdfs:subClassOf fabula:Transfer .

    fabula:Kick
          a       owl:Class ;
          rdfs:comment "Kick an object using ones legs." ;
          rdfs:subClassOf fabula:Attack .

    fabula:InternalAttribute
          a       owl:Class ;
          rdfs:comment "Property made into a class" .

    fabula:GroundMove
          a       owl:Class ;
          rdfs:comment """All move actions that are done over the ground (i.e. a GroundWay) fall in this
category.""" ;
          rdfs:subClassOf fabula:TransitMove .

    fabula:TestMove1
          a       fabula:TestMove ;
          fabula:effects fabula:TestMove1Effects ;
          fabula:interEffects fabula:TestMove1InterEffects ;
          fabula:preconditions
                  "(swc:fromGeographicArea ?path ?currLoc)" , "(swc:toGeographicArea ?path ?TARGET)" .

    fabula:Punch
          a       owl:Class ;
          rdfs:comment "Attack an object using bare hands." ;
          rdfs:subClassOf fabula:Attack .

    fabula:Climb
          a       owl:Class ;
          rdfs:comment """Movement over ground using arms and legs. Used for crossing a
very steep hill or for crossing a path which is blocked by some large
object (like a Wall).""" ;
          rdfs:subClassOf fabula:GroundMove .

    fabula:phi_causes
          a       owl:ObjectProperty ;
          rdfs:subPropertyOf fabula:causes .

    fabula:interruptableDuration
          a       owl:DatatypeProperty , owl:FunctionalProperty ;
          rdfs:comment "Duration of an action in which it can be interrupted. Only used for TransitMoves." ;
          rdfs:domain fabula:Action ;
          rdfs:range <http://www.w3.org/2001/XMLSchema#string> .

    fabula:PutOn
          a       owl:Class ;
          rdfs:comment """The action of placing an Object from ones Hands atop of another
object.""" ;
          rdfs:subClassOf fabula:Put .

    fabula:SustainGoal
          a       owl:Class ;
          rdfs:comment "A goal to sustain a certain situation or state, i.e. being healthy" ;
          rdfs:subClassOf fabula:Goal .

    fabula:ControlAct
          a       owl:Class ;
          rdfs:comment "Actions involving control" ;
          rdfs:subClassOf fabula:Action .

    fabula:Manipulate
          a       owl:Class ;
          rdfs:comment "General class of actions that change one property of an object." ;
          rdfs:subClassOf fabula:Action .

    fabula:Take
          a       owl:Class ;
          rdfs:comment """The action of changing the location of an object to the grabbing device
of the acting object.""" ;
          rdfs:subClassOf fabula:Transfer .

    <http://www.owl-ontologies.com/StoryWorldCore.owl#ind_GeographicArea.plop.7>
          a       ns1:GeographicArea ;
          fabula:hasContext <http://www.owl-ontologies.com/FabulaKnowledge.owl#ind_BeliefElement.plop.3> ;
          fabula:hasInterpretation
                  <http://www.owl-ontologies.com/StoryWorldCore.owl#ind_GeographicArea.plop.5> .

    fabula:AirMove
          a       owl:Class ;
          rdfs:comment """Transit movement through the air. Note that one can fly through
corridors.""" ;
          rdfs:subClassOf fabula:TransitMove .

    fabula:FabulaElement
          a       owl:Class ;
          rdfs:comment "An element that represents a part of fabula, being that what happens in a story, the actual events and processes" .

    fabula:Make
          a       owl:Class ;
          rdfs:comment """[SUMO] The subclass of Creation in which an individual Artifact or a type of
Artifact is made.""" ;
          rdfs:subClassOf fabula:Creation .

    fabula:delete
          a       owl:DatatypeProperty ;
          rdfs:comment "list of facts to be deleted upon a world change." ;
          rdfs:domain fabula:WorldChanges ;
          rdfs:range <http://www.w3.org/2001/XMLSchema#string> .

    <http://www.owl-ontologies.com/StoryWorldCore.owl#ind_GeographicArea.plop.5>
          a       ns1:GeographicArea .

    fabula:AttainGoal
          a       owl:Class ;
          rdfs:comment "A goal to attain a certain situation / state, i.e. being rich" ;
          rdfs:subClassOf fabula:Goal .

    fabula:Dress
          a       owl:Class ;
          rdfs:comment "Putting on WearableProducts, like Bracelets or Jeans." ;
          rdfs:subClassOf fabula:Put .

    fabula:Perception
          a       owl:Class ;
          rdfs:comment "Describing what a character perceives" ;
          rdfs:subClassOf fabula:FabulaElement .

    fabula:Swim
          a       owl:Class ;
          rdfs:comment "Movement through water by using arms or fins." ;
          rdfs:subClassOf fabula:WaterMove .

    fabula:Hear
          a       owl:Class ;
          rdfs:subClassOf fabula:Perception .

    fabula:See
          a       owl:Class ;
          rdfs:subClassOf fabula:Perception .

    fabula:Attack
          a       owl:Class ;
          rdfs:comment "Try to hurt/damage an object." ;
          rdfs:subClassOf fabula:Action .

    <http://www.owl-ontologies.com/FabulaKnowledge.owl#ind_Eat.plop.11>
          a       fabula:Eat ;
          fabula:agens <http://www.owl-ontologies.com/StoryWorldCore.owl#ind_Humanoid.plop.1> ;
          fabula:patiens <http://www.owl-ontologies.com/StoryWorldCore.owl#ind_FruitOrVegetable.plop.6> ;
          fabula:phi_causes <http://www.owl-ontologies.com/FabulaKnowledge.owl#ind_See.plop.12> .

    fabula:Tie
          a       owl:Class ;
          rdfs:comment "Attach one object to another using a rope-like device." ;
          rdfs:subClassOf fabula:Attach .

    <http://www.owl-ontologies.com/FabulaKnowledge.owl#ind_Eat.plop.13>
          a       fabula:Eat ;
          fabula:agens <http://www.owl-ontologies.com/StoryWorldCore.owl#ind_Humanoid.plop.1> ;
          fabula:hasContext <http://www.owl-ontologies.com/FabulaKnowledge.owl#ind_See.plop.12> ;
          fabula:isSuccessful "true" ;
          fabula:patiens <http://www.owl-ontologies.com/StoryWorldCore.owl#ind_FruitOrVegetable.plop.4> .

    fabula:Undress
          a       owl:Class ;
          rdfs:comment "The act of taking off WearableProducts." ;
          rdfs:subClassOf fabula:Take .

    fabula:Attach
          a       owl:Class ;
          rdfs:comment "Attach one object to another using a AttachingDevice." ;
          rdfs:subClassOf fabula:Attaching .

    fabula:ForcefulDetach
          a       owl:Class ;
          rdfs:comment """Detaching an object using force. This can be done on
glued and tied objects. There is the risk of breaking one of the objects,
however.""" ;
          rdfs:subClassOf fabula:Detach .

    <http://www.owl-ontologies.com/FabulaKnowledge.owl#ind_Eat.plop.15>
          a       fabula:Eat ;
          fabula:agens <http://www.owl-ontologies.com/StoryWorldCore.owl#ind_Humanoid.plop.1> ;
          fabula:hasContext <http://www.owl-ontologies.com/FabulaKnowledge.owl#ind_BeliefElement.plop.14> ;
          fabula:patiens <http://www.owl-ontologies.com/StoryWorldCore.owl#ind_FruitOrVegetable.plop.6> ;
          fabula:sameConcept <http://www.owl-ontologies.com/FabulaKnowledge.owl#ind_Eat.plop.13> .

    fabula:Strike
          a       owl:Class ;
          rdfs:comment "Attack an object while holding another object to hit with. (i.e. use that object as weapon)." ;
          rdfs:subClassOf fabula:Attack .

    <http://www.owl-ontologies.com/FabulaKnowledge.owl#ind_Hunger.plop.2>
          fabula:character <http://www.owl-ontologies.com/StoryWorldCore.owl#ind_Humanoid.plop.1> ;
          fabula:psi_causes <http://www.owl-ontologies.com/StoryWorldCore.owl#ind_AttainGoal.plop.8> .

    fabula:Run
          a       owl:Class ;
          rdfs:comment """Fast movement over ground. Consumes more energy per distance
measure.""" ;
          rdfs:subClassOf fabula:Ambulate .

    fabula:Drive
          a       owl:Class ;
          rdfs:comment "Movement over ground by means of Wheels." ;
          rdfs:subClassOf fabula:GroundMove .

    <http://www.owl-ontologies.com/StoryWorldCore.owl#ind_Humanoid.plop.1>
          a       ns1:Humanoid .

    fabula:Sail
          a       owl:Class ;
          rdfs:comment """Movement through water by means of transportation device. Can be
split in movement needing wind and movement using an engine.""" ;
          rdfs:subClassOf fabula:WaterMove .
}

